step 4: pull packet number out of Impl header

src/QUIC.Impl.Base.fst
@@ -17,22 +17,23 @@ module Spec = QUIC.Spec.Base
 length of the actual payload, NOT including the length of the packet
 number. *)
 
+(* NOTE: the header no longer contains the packet number, which is
+part of the state, so that the client no longer needs to take care of
+it *)
+
 noeq type long_header_specifics =
   | BInitial:
     payload_length: uint62_t ->
-    packet_number: uint62_t ->
     (packet_number_length: packet_number_length_t { U64.v payload_length + U32.v packet_number_length < pow2 62 }) ->
     token: B.buffer U8.t -> (* I reordered those so that the extracted code for this type is a tagged union with common prefixes *)
     token_length: U32.t { let v = U32.v token_length in v == B.length token /\ 0 <= v /\ v <= token_max_len  } ->
     long_header_specifics
   | BZeroRTT:
     payload_length: uint62_t ->
-    packet_number: uint62_t ->
     (packet_number_length: packet_number_length_t { U64.v payload_length + U32.v packet_number_length < pow2 62 }) ->
     long_header_specifics
   | BHandshake:
     payload_length: uint62_t ->
-    packet_number: uint62_t ->
     (packet_number_length: packet_number_length_t { U64.v payload_length + U32.v packet_number_length < pow2 62 }) ->
     long_header_specifics
   | BRetry:
@@ -59,7 +60,6 @@ noeq type header =
       l == B.length cid /\
       0 <= l /\ l <= 20
     } ->
-    packet_number: uint62_t ->
     packet_number_length: packet_number_length_t ->
     header
 
@@ -67,12 +67,12 @@ module HS = FStar.HyperStack
 
 let header_live (h: header) (m: HS.mem) : GTot Type0 =
   match h with
-  | BShort spin phase cid cid_len packet_number packet_number_length ->
+  | BShort spin phase cid cid_len packet_number_length ->
     B.live m cid
   | BLong version dcid dcil scid scil spec ->
     B.live m dcid /\ B.live m scid /\
     begin match spec with
-    | BInitial payload_length packet_number packet_number_length token token_length ->
+    | BInitial payload_length packet_number_length token token_length ->
       B.live m token
     | BRetry unused odcid odcil ->
       B.live m odcid
@@ -81,12 +81,12 @@ let header_live (h: header) (m: HS.mem) : GTot Type0 =
 
 let header_footprint (h: header) : GTot B.loc =
   match h with
-  | BShort spin phase cid cid_len packet_number packet_number_length ->
+  | BShort spin phase cid cid_len packet_number_length ->
     B.loc_buffer cid
   | BLong version dcid dcil scid scil spec ->
     (B.loc_buffer dcid `B.loc_union` B.loc_buffer scid) `B.loc_union`
     begin match spec with
-    | BInitial payload_length packet_number packet_number_length token token_length ->
+    | BInitial payload_length packet_number_length token token_length ->
       B.loc_buffer token
     | BRetry unused odcid odcil ->
       B.loc_buffer odcid
@@ -95,18 +95,18 @@ let header_footprint (h: header) : GTot B.loc =
 
 module FB = FStar.Bytes
 
-let g_header (h: header) (m: HS.mem) : GTot Spec.header =
+let g_header (h: header) (m: HS.mem) (packet_number: uint62_t) : GTot Spec.header =
   match h with
-  | BShort spin phase cid cid_len packet_number packet_number_length ->
+  | BShort spin phase cid cid_len packet_number_length ->
     MShort spin phase (FB.hide (B.as_seq m cid)) packet_number_length packet_number
   | BLong version dcid dcil scid scil spec ->
     MLong version (FB.hide (B.as_seq m dcid)) (FB.hide (B.as_seq m scid))
       begin match spec with
-      | BInitial payload_length packet_number packet_number_length token token_length ->
+      | BInitial payload_length packet_number_length token token_length ->
         MInitial (FB.hide (B.as_seq m token)) payload_length packet_number_length packet_number
-      | BZeroRTT payload_length packet_number packet_number_length ->
+      | BZeroRTT payload_length packet_number_length ->
         MZeroRTT payload_length packet_number_length packet_number
-      | BHandshake payload_length packet_number packet_number_length ->
+      | BHandshake payload_length packet_number_length ->
         MHandshake payload_length packet_number_length packet_number
       | BRetry unused odcid odcil ->
         MRetry unused (FB.hide (B.as_seq m odcid))
@@ -114,11 +114,12 @@ let g_header (h: header) (m: HS.mem) : GTot Spec.header =
 
 let frame_header
   (h: header)
+  (packet_number: uint62_t)
   (l: B.loc)
   (m1 m2: HS.mem)
 : Lemma
   (requires (header_live h m1 /\ B.modifies l m1 m2 /\ B.loc_disjoint l (header_footprint h)))
-  (ensures (header_live h m2 /\ g_header h m2 == g_header h m1))
+  (ensures (header_live h m2 /\ g_header h m2 packet_number == g_header h m1 packet_number))
 = ()
 
 (* Length computations need to be transparent because the precondition
@@ -144,16 +145,16 @@ let header_len
   (h: header)
 : Tot U32.t
 = match h with
-  | BShort spin phase cid cid_len packet_number packet_number_length ->
+  | BShort spin phase cid cid_len packet_number_length ->
     1ul `U32.add` cid_len `U32.add` packet_number_length
   | BLong version dcid dcil scid scil spec ->
     7ul `U32.add` dcil `U32.add` scil `U32.add`
     begin match spec with
-    | BInitial payload_length packet_number packet_number_length token token_length ->
+    | BInitial payload_length packet_number_length token token_length ->
       varint_len (Cast.uint32_to_uint64 token_length) `U32.add` token_length `U32.add` varint_len payload_length `U32.add` packet_number_length
-    | BZeroRTT payload_length packet_number packet_number_length ->
+    | BZeroRTT payload_length packet_number_length ->
       varint_len payload_length `U32.add` packet_number_length
-    | BHandshake payload_length packet_number packet_number_length ->
+    | BHandshake payload_length packet_number_length ->
       varint_len payload_length `U32.add` packet_number_length
     | BRetry unused odcid odcil ->
       1ul `U32.add` odcil
