src/QUIC.Impl.Header.fsti
@@ -17,7 +17,7 @@ val read_header
   (packet_len: U32.t { let v = U32.v packet_len in v == B.length packet /\ v < 4294967280 })
   (cid_len: U32.t { U32.v cid_len < 20 } )
   (last: uint62_t { U64.v last + 1 < pow2 62 })
-: HST.Stack (option (Impl.header & U32.t))
+: HST.Stack (option (Impl.header & uint62_t & U32.t))
   (requires (fun h ->
     B.live h packet
   ))
@@ -27,14 +27,14 @@ val read_header
       let spec = parse_header (U32.v cid_len) (U64.v last) (B.as_seq h packet) in
       match res with
       | None -> H_Failure? spec
-      | Some (x, len) ->
+      | Some (x, pn, len) ->
         H_Success? spec /\
         begin
           let H_Success hd _ = spec in
           Impl.header_live x h' /\
           U32.v len <= B.length packet /\
           B.loc_buffer (B.gsub packet 0ul len) `B.loc_includes` Impl.header_footprint x /\
-          Impl.g_header x h' == hd /\
+          Impl.g_header x h' pn == hd /\
           U32.v len = Spec.header_len hd
         end
     end
@@ -43,16 +43,17 @@ val read_header
 val write_header
   (dst: B.buffer U8.t)
   (x: Impl.header)
+  (pn: uint62_t)
 : HST.Stack unit
   (requires (fun h ->
     B.live h dst /\
     Impl.header_live x h /\
-    B.length dst == Spec.header_len (Impl.g_header x h) /\
+    B.length dst == Spec.header_len (Impl.g_header x h pn) /\
     Impl.header_footprint x `B.loc_disjoint` B.loc_buffer dst
   ))
   (ensures (fun h _ h' ->
     B.modifies (B.loc_buffer dst) h h' /\
-    B.as_seq h' dst == format_header (Impl.g_header x h)
+    B.as_seq h' dst == format_header (Impl.g_header x h pn)
   ))
 
 val putative_pn_offset
@@ -77,14 +78,15 @@ val putative_pn_offset
 
 val pn_offset
   (h: Impl.header)
+  (pn: Ghost.erased uint62_t)
 : HST.Stack U32.t
   (requires (fun m ->
     Impl.header_live h m /\
-    (~ (is_retry (Impl.g_header h m)))
+    (~ (is_retry (Impl.g_header h m (Ghost.reveal pn))))
   ))
   (ensures (fun m res m' ->
     B.modifies B.loc_none m m' /\
-    U32.v res == pn_offset (Impl.g_header h m)
+    U32.v res == pn_offset (Impl.g_header h m (Ghost.reveal pn))
   ))
 
 module HS = FStar.HyperStack
@@ -92,5 +94,6 @@ module HS = FStar.HyperStack
 val header_len_correct
   (h: Impl.header)
   (m: HS.mem)
+  (pn: uint62_t)
 : Lemma
-  (U32.v (Impl.header_len h) == Spec.header_len (Impl.g_header h m))
+  (U32.v (Impl.header_len h) == Spec.header_len (Impl.g_header h m pn))
